CapDL: Made IRQ Nodes a new object type, not a small CNode.
IRQ Nodes are now their own object type in capDL. This makes it much easier
to distinguish between "real" CNodes and IRQ Nodes.

Updated:
 * the capDL refinement,
 * the access proofs, and
 * the system initialiser.

spec/capDL/Types_D.thy
@@ -190,6 +190,9 @@ record cdl_page_directory =
 record cdl_frame =
   cdl_frame_size_bits :: cdl_size_bits
 
+record cdl_irq_node =
+  cdl_irq_node_caps :: cdl_cap_map
+
 (*
  * Kernel objects.
  *
@@ -206,6 +209,7 @@ datatype cdl_object =
   | PageDirectory cdl_page_directory
   | Frame cdl_frame
   | Untyped
+  | IRQNode cdl_irq_node
 
 (* The architecture that we are modelling. *)
 datatype cdl_arch = IA32 | ARM11
@@ -267,6 +271,7 @@ where
       | AsyncEndpoint \<Rightarrow> AsyncEndpointType
       | Tcb _ \<Rightarrow> TcbType
       | CNode _ \<Rightarrow> CNodeType
+      | IRQNode _ \<Rightarrow> IRQNodeType
       | AsidPool _ \<Rightarrow> AsidPoolType
       | PageTable _ \<Rightarrow> PageTableType
       | PageDirectory _ \<Rightarrow> PageDirectoryType
@@ -449,6 +454,7 @@ where
   | AsidPool x \<Rightarrow> cdl_asid_pool_caps x
   | CNode x \<Rightarrow> cdl_cnode_caps x
   | Tcb x \<Rightarrow> cdl_tcb_caps x
+  | IRQNode x \<Rightarrow> cdl_irq_node_caps x
   | _ \<Rightarrow> empty"
 
 definition
@@ -460,6 +466,7 @@ where
   | AsidPool x \<Rightarrow> AsidPool (x\<lparr>cdl_asid_pool_caps := new_val\<rparr>)
   | CNode x \<Rightarrow> CNode (x\<lparr>cdl_cnode_caps := new_val\<rparr>)
   | Tcb x \<Rightarrow> Tcb (x\<lparr>cdl_tcb_caps := new_val\<rparr>)
+  | IRQNode x \<Rightarrow> IRQNode (x\<lparr>cdl_irq_node_caps := new_val\<rparr>)
   | _ \<Rightarrow> obj"
 
 definition
@@ -471,6 +478,7 @@ where
   | AsidPool _ \<Rightarrow> True
   | CNode _ \<Rightarrow> True
   | Tcb _ \<Rightarrow> True
+  | IRQNode _ \<Rightarrow> True
   | _ \<Rightarrow> False"
 
 
@@ -513,6 +521,7 @@ where
   | PageTableCap _ _ _     \<Rightarrow> Some PageTableType
   | PageDirectoryCap _ _ _ \<Rightarrow> Some PageDirectoryType
   | FrameCap _ _ f _ _     \<Rightarrow> Some (FrameType f)
+  | IrqHandlerCap _        \<Rightarrow> Some IRQNodeType
   | _                      \<Rightarrow> None "
 
 abbreviation "is_untyped_cap cap    \<equiv> (cap_type cap = Some UntypedType)"
@@ -524,7 +533,7 @@ abbreviation "is_asidpool_cap cap   \<equiv> (cap_type cap = Some AsidPoolType)"
 abbreviation "is_pt_cap cap         \<equiv> (cap_type cap = Some PageTableType)"
 abbreviation "is_pd_cap cap         \<equiv> (cap_type cap = Some PageDirectoryType)"
 abbreviation "is_frame_cap cap      \<equiv> (\<exists>sz. cap_type cap = Some (FrameType sz))"
-definition   "is_irqhandler_cap cap \<equiv> (case cap of IrqHandlerCap _ \<Rightarrow> True | _ \<Rightarrow> False)"
+abbreviation "is_irqhandler_cap cap \<equiv> (cap_type cap = Some IRQNodeType)"
 definition   "is_irqcontrol_cap cap \<equiv> (cap = IrqControlCap)"
 
 lemma cap_type_simps [simp]:
@@ -538,11 +547,8 @@ lemma cap_type_simps [simp]:
   "is_pt_cap         (PageTableCap u v w)"
   "is_frame_cap      (FrameCap a1 a2 a3 a4 a5)"
   "is_irqhandler_cap (IrqHandlerCap a6)"
-  by (clarsimp simp: cap_type_def is_irqhandler_cap_def)+
-
-lemma is_irqhandler_cap_cap_type [simp]:
-  "is_irqhandler_cap cap \<Longrightarrow> cap_type cap = None"
-  by (clarsimp simp: is_irqhandler_cap_def cap_type_def split: cdl_cap.splits)
+  "cap_type (FrameCap obj_id rights sz rs asid) = Some (FrameType sz)"
+  by (clarsimp simp: cap_type_def)+
 
 abbreviation "cap_has_type cap \<equiv> (\<exists>type. cap_type cap = Some type)"
 
@@ -593,9 +599,9 @@ where
   "empty_cnode sz = \<lparr> cdl_cnode_caps = empty_cap_map sz, cdl_cnode_size_bits = sz \<rparr>"
 
 definition
-  empty_irq_node :: cdl_object
+  empty_irq_node :: cdl_irq_node
 where
-  "empty_irq_node \<equiv> CNode (empty_cnode 0)"
+  "empty_irq_node \<equiv> \<lparr> cdl_irq_node_caps = empty_cap_map 0 \<rparr>"
 
 (* Standard empty TCB object. *)
 definition
@@ -629,7 +635,8 @@ where
       | AsidPoolType \<Rightarrow> Some (AsidPool \<lparr> cdl_asid_pool_caps = empty_cap_map asid_low_bits \<rparr>)
       | PageTableType \<Rightarrow> Some (PageTable \<lparr> cdl_page_table_caps = empty_cap_map 8 \<rparr>)
       | PageDirectoryType \<Rightarrow> Some (PageDirectory \<lparr> cdl_page_directory_caps = empty_cap_map 12 \<rparr>)
-      | FrameType sz \<Rightarrow> Some (Frame \<lparr> cdl_frame_size_bits = sz \<rparr>)"
+      | FrameType sz \<Rightarrow> Some (Frame \<lparr> cdl_frame_size_bits = sz \<rparr>)
+      | IRQNodeType \<Rightarrow> Some (IRQNode empty_irq_node)"
 
 abbreviation "pick a \<equiv> SOME x. x\<in> a"
 
@@ -643,6 +650,7 @@ where
       | AsyncEndpointType \<Rightarrow> AsyncEndpointCap (THE i. i \<in> id_set) 0 {Read,Write}
       | TcbType \<Rightarrow> TcbCap (pick id_set)
       | CNodeType \<Rightarrow> CNodeCap (pick id_set) 0 0 sz
+      | IRQNodeType \<Rightarrow> IrqHandlerCap undefined
       | UntypedType \<Rightarrow> UntypedCap id_set id_set
       | AsidPoolType \<Rightarrow> AsidPoolCap (pick id_set) (0, 0)
       | PageTableType \<Rightarrow> PageTableCap (pick id_set) Real None
